Subtyping.v
@@ -92,8 +92,6 @@ Qed.
 Lemma qualified_type_subtype_base_subtype :
   forall CT qt1 qt2,
     qualified_type_subtype CT qt1 qt2 ->
-    (sctype qt1) < (dom CT) ->
-    (sctype qt2) < (dom CT) ->
     base_subtype CT (sctype qt1) (sctype qt2).
 Proof.
     intros CT qt1 qt2 H.
@@ -101,12 +99,7 @@ Proof.
     generalize dependent qt1.
     generalize dependent qt2.
     - intros. exact H2.
-    - 
-      intros Hf1 Hf3.
-      apply qualified_type_subtype_dom2 in H as Hf2.
-      pose proof IHqualified_type_subtype1 Hf1 Hf2 as B1.
-      pose proof IHqualified_type_subtype2 Hf2 Hf3 as B2.
-      exact (base_trans _ _ _ _ B1 B2).
+    - eapply base_trans; eauto. 
     - 
 			intros. apply base_refl.
 			exact H.
@@ -115,8 +108,6 @@ Qed.
 Lemma qualified_type_subtype_q_subtype :
   forall CT qt1 qt2,
     qualified_type_subtype CT qt1 qt2 ->
-    (sctype qt1) < (dom CT) ->
-    (sctype qt2) < (dom CT) ->
     q_subtype (sqtype qt1) (sqtype qt2).
 Proof.
   intros CT qt1 qt2 H.
@@ -124,11 +115,7 @@ Proof.
   - (* qtype_sub case *)
     intros. exact H1.
   - (* qtype_trans case *)
-  intros Hf1 Hf3.
-  apply qualified_type_subtype_dom2 in H as Hf2.
-  pose proof IHqualified_type_subtype1 Hf1 Hf2 as Q1.
-  pose proof IHqualified_type_subtype2 Hf2 Hf3 as Q2.
-  exact (q_subtype_trans _ _ _ Q1 Q2).  
+  eapply q_subtype_trans; eauto.
   - (* qtype_refl case *)
     intros. 
     destruct qt as [q c]; simpl.
