Todoproperty.v
@@ -778,3 +778,936 @@ Proof.
       exists rΓ' h'. right. apply SBS_Seq_NPE_first; assumption.
 Admitted.
 Qed. *)
+
+
+  (* 6: 
+  {
+    inversion Htyping; subst.
+    remember (mreceiver m_sig :: mparams m_sig) as sΓmethodinit.
+    remember {| vars := Iot ly :: vals |} as rΓmethodinit.
+    remember (rΓ <| vars := update x retval (vars rΓ) |>) as rΓ'''.
+    apply method_sig_lookup_implies_body_lookup in H16.
+    destruct H16 as [mbody0 H16].
+    apply method_body_lookup_implies_def_lookup in H16.
+    destruct H16 as [mdef H16].
+    destruct H16 as [Hmdef_lookup Hbody_eq].
+    apply method_body_well_typed in Hmdef_lookup; auto.
+    destruct Hmdef_lookup as [sΓmethodend Hmdef_lookup].
+    assert (wf_r_config CT sΓmethodend rΓ'' h'). {
+      eapply IHHeval with (sΓ := sΓmethodinit) (sΓ' := sΓmethodend); eauto.
+      admit.
+      admit. (* with some rewrite *)
+      (* exact Hmdef_lookup. *)
+    }
+    admit.
+    unfold wf_r_config in Hwf.
+    destruct Hwf as [Hwf_classtable _].
+    exact Hwf_classtable.
+    generalize dependent sΓ'.
+    induction H9; try discriminate.
+    6:{(* method call case again*)
+      intros.
+      subst.
+      apply IHeval_stmt.
+      Print IHeval_stmt.
+      (* apply IHeval_stmt with (mbody:=mbody0). *)
+      (* apply IHeval_stmt with (mbody1:=mbody0). *)
+      all: try reflexivity.
+      exact H.
+      exact H3.
+      exact H5.
+      exact H6.
+      exact H7.
+      exact H8.
+      exact H9.
+      exact H15.
+      exact H16.
+      admit.
+      admit.
+      admit.
+      exact Hwf_method_frame.
+    }
+    {
+      unfold wf_r_config in *.
+      destruct H8 as [Hclass [Hheap [Hrenv [Hsenv [Hlen Hcorr]]]]].
+      destruct Hclass as [Hclass [Hobj [Hotherclasses Hcname_consistent]]].
+      repeat split.
+      unfold wf_class_table in Hclass.
+      exact Hclass.
+      exact Hobj.
+      exact Hotherclasses.
+      apply Hcname_consistent.
+      apply Hcname_consistent.
+      subst.
+      exact Hheap.
+      unfold wf_renv in Hrenv.
+      destruct Hrenv as [HrEnvLen [Hreceiverval Hallvals]].
+      simpl.
+      subst rΓ'.
+      rewrite update_length.
+      exact HrEnvLen.
+      unfold wf_renv in Hrenv.
+      destruct Hrenv as [HrEnvLen [Hreceiverval Hallvals]].
+      destruct Hreceiverval as [iot [Hiot Hiotdom]].
+      exists iot.
+      simpl.
+      unfold gget in *.
+      {destruct (vars rΓ) as [|v0 vs] eqn:Hvars.
+      - (* Case: vars rΓ = [] *)
+        exfalso.
+        simpl in HrEnvLen.
+        lia.
+      - (* Case: vars rΓ = v0 :: vs *)
+        destruct x as [|x'].
+        + (* Case: x = 0 *)
+          contradiction H4.
+          reflexivity.
+        + (* Case: x = S x' *)
+          simpl.
+          split.
+          * subst rΓ'. exact Hiot.
+          * exact Hiotdom.
+      }
+      {
+        unfold wf_renv in Hrenv.
+        destruct Hrenv as [HrEnvLen [Hreceiverval Hallvals]].
+        simpl.
+        subst rΓ'.
+        apply Forall_update.
+        exact Hallvals.
+        destruct retval as [|loc]. easy.
+        subst.
+        admit.
+        apply static_getType_dom in H0.
+        rewrite <- Hlen.
+        exact H0.
+      }
+      destruct Hsenv as [HsenvLength HsenvWellTyped].
+      exact HsenvLength.
+      destruct Hsenv as [HsenvLength HsenvWellTyped].
+      exact HsenvWellTyped.
+      subst rΓ'.
+      rewrite update_length.
+      exact Hlen.
+      admit.
+    }
+    {
+      unfold wf_r_config in *.
+      destruct H8 as [Hclass [Hheap [Hrenv [Hsenv [Hlen Hcorr]]]]].
+      repeat split.
+      unfold wf_class_table in Hclass.
+      destruct Hclass as [Hclass [Hobj [Hotherclasses Hcname_consistent]]].
+      exact Hclass.
+      destruct Hclass as [Hclass [Hobj [Hotherclasses Hcname_consistent]]].
+      exact Hobj.
+      destruct Hclass as [Hclass [Hobj [Hotherclasses Hcname_consistent]]].
+      exact Hotherclasses.
+      destruct Hclass as [Hclass [Hobj [Hotherclasses Hcname_consistent]]].
+      apply Hcname_consistent.
+      destruct Hclass as [Hclass [Hobj [Hotherclasses Hcname_consistent]]].
+      apply Hcname_consistent.
+      exact Hheap. 
+      unfold wf_renv in Hrenv.
+      destruct Hrenv as [HrEnvLen [Hreceiverval Hallvals]].
+      simpl.
+      subst rΓ'.
+      rewrite update_length.
+      exact HrEnvLen.
+      unfold wf_renv in Hrenv.
+      destruct Hrenv as [HrEnvLen [Hreceiverval Hallvals]].
+      destruct Hreceiverval as [iot [Hiot Hiotdom]].
+      exists iot.
+      simpl.
+      unfold gget in *.
+      {destruct (vars rΓ) as [|v0 vs] eqn:Hvars.
+      - (* Case: vars rΓ = [] *)
+        exfalso.
+        simpl in HrEnvLen.
+        lia.
+      - (* Case: vars rΓ = v0 :: vs *)
+        destruct x as [|x'].
+        + (* Case: x = 0 *)
+          contradiction H4.
+          reflexivity.
+        + (* Case: x = S x' *)
+          simpl.
+          split.
+          * subst rΓ'. exact Hiot.
+          * exact Hiotdom.
+      }
+      {
+        unfold wf_renv in Hrenv.
+        destruct Hrenv as [HrEnvLen [Hreceiverval Hallvals]].
+        simpl.
+        subst rΓ'.
+        apply Forall_update.
+        exact Hallvals.
+        destruct retval as [|loc]. easy.
+        admit.
+        apply static_getType_dom in H0.
+        rewrite <- Hlen.
+        exact H0.
+      }
+      destruct Hsenv as [HsenvLength HsenvWellTyped].
+      exact HsenvLength.
+      destruct Hsenv as [HsenvLength HsenvWellTyped].
+      exact HsenvWellTyped.
+      subst rΓ'.
+      rewrite update_length.
+      exact Hlen.
+      admit.
+    }
+    {
+      unfold wf_r_config in *.
+      destruct H8 as [Hclass [Hheap [Hrenv [Hsenv [Hlen Hcorr]]]]].
+      repeat split.
+      unfold wf_class_table in Hclass.
+      destruct Hclass as [Hclass [Hobj [Hotherclasses Hcname_consistent]]].
+      exact Hclass.
+      destruct Hclass as [Hclass [Hobj [Hotherclasses Hcname_consistent]]].
+      exact Hobj.
+      destruct Hclass as [Hclass [Hobj [Hotherclasses Hcname_consistent]]].
+      exact Hotherclasses.
+      destruct Hclass as [Hclass [Hobj [Hotherclasses Hcname_consistent]]].
+      apply Hcname_consistent.
+      destruct Hclass as [Hclass [Hobj [Hotherclasses Hcname_consistent]]].
+      apply Hcname_consistent.
+      exact Hheap. 
+      unfold wf_renv in Hrenv.
+      destruct Hrenv as [HrEnvLen [Hreceiverval Hallvals]].
+      simpl.
+      subst rΓ'.
+      rewrite update_length.
+      exact HrEnvLen.
+      unfold wf_renv in Hrenv.
+      destruct Hrenv as [HrEnvLen [Hreceiverval Hallvals]].
+      destruct Hreceiverval as [iot [Hiot Hiotdom]].
+      exists iot.
+      simpl.
+      unfold gget in *.
+      {destruct (vars rΓ) as [|v0 vs] eqn:Hvars.
+      - (* Case: vars rΓ = [] *)
+        exfalso.
+        simpl in HrEnvLen.
+        lia.
+      - (* Case: vars rΓ = v0 :: vs *)
+        destruct x as [|x'].
+        + (* Case: x = 0 *)
+          contradiction H4.
+          reflexivity.
+        + (* Case: x = S x' *)
+          simpl.
+          split.
+          * subst rΓ'. exact Hiot.
+          * exact Hiotdom.
+      }
+      {
+        unfold wf_renv in Hrenv.
+        destruct Hrenv as [HrEnvLen [Hreceiverval Hallvals]].
+        simpl.
+        subst rΓ'.
+        apply Forall_update.
+        exact Hallvals.
+        destruct retval as [|loc]. easy.
+        admit.
+        apply static_getType_dom in H0.
+        rewrite <- Hlen.
+        exact H0.
+      }
+      destruct Hsenv as [HsenvLength HsenvWellTyped].
+      exact HsenvLength.
+      destruct Hsenv as [HsenvLength HsenvWellTyped].
+      exact HsenvWellTyped.
+      subst rΓ'.
+      rewrite update_length.
+      exact Hlen.
+      admit.
+    }
+    {
+      unfold wf_r_config in *.
+      destruct H8 as [Hclass [Hheap [Hrenv [Hsenv [Hlen Hcorr]]]]].
+      repeat split.
+      unfold wf_class_table in Hclass.
+      destruct Hclass as [Hclass [Hobj [Hotherclasses Hcname_consistent]]].
+      exact Hclass.
+      destruct Hclass as [Hclass [Hobj [Hotherclasses Hcname_consistent]]].
+      exact Hobj.
+      destruct Hclass as [Hclass [Hobj [Hotherclasses Hcname_consistent]]].
+      exact Hotherclasses.
+      destruct Hclass as [Hclass [Hobj [Hotherclasses Hcname_consistent]]].
+      apply Hcname_consistent.
+      destruct Hclass as [Hclass [Hobj [Hotherclasses Hcname_consistent]]].
+      apply Hcname_consistent.
+      (* exact Hheap.  *)
+      admit.
+      unfold wf_renv in Hrenv.
+      destruct Hrenv as [HrEnvLen [Hreceiverval Hallvals]].
+      simpl.
+      subst rΓ'.
+      rewrite update_length.
+      exact HrEnvLen.
+      unfold wf_renv in Hrenv.
+      destruct Hrenv as [HrEnvLen [Hreceiverval Hallvals]].
+      destruct Hreceiverval as [iot [Hiot Hiotdom]].
+      exists iot.
+      simpl.
+      unfold gget in *.
+      {destruct (vars rΓ) as [|v0 vs] eqn:Hvars.
+      - (* Case: vars rΓ = [] *)
+        exfalso.
+        simpl in HrEnvLen.
+        lia.
+      - (* Case: vars rΓ = v0 :: vs *)
+        destruct x as [|x'].
+        + (* Case: x = 0 *)
+          contradiction H4.
+          reflexivity.
+        + (* Case: x = S x' *)
+          simpl.
+          split.
+          * subst rΓ'. exact Hiot.
+          * subst h'. rewrite update_field_length. exact Hiotdom.
+      }
+      {
+        unfold wf_renv in Hrenv.
+        destruct Hrenv as [HrEnvLen [Hreceiverval Hallvals]].
+        simpl.
+        subst rΓ'.
+        apply Forall_update.
+        admit.
+        admit.
+        (* exact Hallvals.
+        destruct retval as [|loc]. easy. *)
+        apply static_getType_dom in H0.
+        rewrite <- Hlen.
+        exact H0.
+      }
+      destruct Hsenv as [HsenvLength HsenvWellTyped].
+      exact HsenvLength.
+      destruct Hsenv as [HsenvLength HsenvWellTyped].
+      exact HsenvWellTyped.
+      subst rΓ'.
+      rewrite update_length.
+      exact Hlen.
+      admit.
+    }
+    { (* Object creation case *)
+      unfold wf_r_config in *.
+      destruct H8 as [Hclass [Hheap [Hrenv [Hsenv [Hlen Hcorr]]]]].
+      repeat split.
+      unfold wf_class_table in Hclass.
+      destruct Hclass as [Hclass [Hobj [Hotherclasses Hcname_consistent]]].
+      exact Hclass.
+      destruct Hclass as [Hclass [Hobj [Hotherclasses Hcname_consistent]]].
+      exact Hobj.
+      destruct Hclass as [Hclass [Hobj [Hotherclasses Hcname_consistent]]].
+      exact Hotherclasses.
+      destruct Hclass as [Hclass [Hobj [Hotherclasses Hcname_consistent]]].
+      apply Hcname_consistent.
+      destruct Hclass as [Hclass [Hobj [Hotherclasses Hcname_consistent]]].
+      apply Hcname_consistent.
+      admit.
+      (* exact Hheap.  *)
+      unfold wf_renv in Hrenv.
+      destruct Hrenv as [HrEnvLen [Hreceiverval Hallvals]].
+      simpl.
+      subst rΓ'.
+      rewrite update_length.
+      exact HrEnvLen.
+      unfold wf_renv in Hrenv.
+      destruct Hrenv as [HrEnvLen [Hreceiverval Hallvals]].
+      destruct Hreceiverval as [iot [Hiot Hiotdom]].
+      exists iot.
+      simpl.
+      unfold gget in *.
+      {destruct (vars rΓ) as [|v0 vs] eqn:Hvars.
+      - (* Case: vars rΓ = [] *)
+        exfalso.
+        simpl in HrEnvLen.
+        lia.
+      - (* Case: vars rΓ = v0 :: vs *)
+        destruct x as [|x'].
+        + (* Case: x = 0 *)
+          contradiction H4.
+          reflexivity.
+        + (* Case: x = S x' *)
+          simpl.
+          split.
+          * subst rΓ'. exact Hiot.
+          * subst h'.
+            rewrite length_app.
+            simpl.
+            lia.
+      }
+      {
+        unfold wf_renv in Hrenv.
+        destruct Hrenv as [HrEnvLen [Hreceiverval Hallvals]].
+        simpl.
+        subst rΓ'.
+        apply Forall_update.
+        subst.
+        (* exact Hallvals. *)
+        (* destruct retval as [|loc]. easy. *)
+        admit.
+        admit.
+        apply static_getType_dom in H0.
+        rewrite <- Hlen.
+        exact H0.
+      }
+      destruct Hsenv as [HsenvLength HsenvWellTyped].
+      exact HsenvLength.
+      destruct Hsenv as [HsenvLength HsenvWellTyped].
+      exact HsenvWellTyped.
+      subst rΓ'.
+      rewrite update_length.
+      exact Hlen.
+      admit.
+    }
+    { (* sequence case *)
+      subst.
+      admit.
+    }
+  } *)
+
+
+(* Lemma eval_stmt_preserves_heap_domain : forall CT sΓ sΓ' rΓ h stmt rΓ' h',
+  wf_r_config CT sΓ rΓ h ->
+  stmt_typing CT sΓ stmt sΓ' -> 
+  eval_stmt OK CT rΓ h stmt OK rΓ' h' ->
+  dom h <= dom h'.
+Proof.
+  intros CT sΓ sΓ' rΓ h stmt rΓ' h' Hwf Hstmttyping Heval.
+  generalize dependent sΓ.
+  generalize dependent sΓ'.
+  remember OK as ok; induction Heval; try reflexivity; try discriminate.
+  3:{
+    intros.
+    apply method_body_lookup_implies_def_lookup in H1.
+    destruct H1 as [mdef H1].
+    remember (msignature mdef) as msig.
+    destruct H1 as [Hmdef_lookup Hbody_eq].
+    have Hmdef_lookupcopy := Hmdef_lookup. 
+    apply method_body_well_typed in Hmdef_lookup; auto.
+    destruct Hmdef_lookup as [sΓmethodend Hmdef_lookup].
+    remember (mreceiver (msignature mdef) :: mparams (msignature mdef)) as sΓmethodinit.
+    apply IHHeval with (sΓ:=sΓmethodinit)(sΓ':=sΓmethodend); auto.
+    assert (Hwf_method_frame : wf_r_config CT sΓmethodinit 
+                                     rΓ' h).
+    {
+      unfold wf_r_config in *.
+      destruct Hwf as [Hclass [Hheap [Hrenv [Hsenv [Hlen Hcorr]]]]].
+      have Hclasstable := Hclass.
+      destruct Hclass as [Hclass [Hobj [Hotherclasses Hcname_consistent]]].
+      repeat split.
+      exact Hclass.
+      exact Hobj.
+      exact Hotherclasses.
+      apply Hcname_consistent.
+      apply Hcname_consistent.
+      exact Hheap.
+      rewrite H5.
+      simpl.
+      lia.
+      unfold wf_renv in Hrenv.
+      destruct Hrenv as [HrEnvLen [Hreceiverval Hallvals]].
+      exists ly.
+      split.
+      rewrite H5.
+      simpl.
+      reflexivity.
+      unfold runtime_getVal in H.
+      destruct (nth_error (vars rΓ) y) as [v|] eqn:Hnth_y; [|discriminate].
+      injection H as H1_eq.
+      subst v.
+      eapply Forall_nth_error in Hallvals; eauto.
+      simpl in Hallvals.
+      destruct (runtime_getObj h ly) as [obj|] eqn:Hobjly; [|contradiction].
+      apply runtime_getObj_dom in Hobjly.
+      exact Hobjly.
+
+      (* Inner runtime env is wellformed*)
+      rewrite H5.
+      simpl.
+      constructor.
+      simpl.
+      unfold runtime_getVal in H.
+      destruct (nth_error (vars rΓ) y) as [v|] eqn:Hnth_y; [|discriminate].
+      injection H as H1_eq.
+      subst v.
+      unfold runtime_getVal in Hnth_y.
+      unfold wf_renv in Hrenv.
+      destruct Hrenv as [_ [_ Hallvals]].
+      eapply Forall_nth_error in Hallvals; eauto.
+      simpl in Hallvals.
+      exact Hallvals.
+      eapply runtime_lookup_list_preserves_wf_values; eauto.
+
+      rewrite HeqsΓmethodinit.
+      simpl.
+      lia.
+      
+      (* Inner static env's elements are wellformed typeuse *)
+      rewrite HeqsΓmethodinit.
+      constructor.
+      (* Receiver type is well-formed *)
+      apply method_sig_wf_from_def with (m_sig := (msignature mdef)) in Hmdef_lookupcopy; auto.
+      destruct Hmdef_lookupcopy as [Hreceiver _].
+      exact Hreceiver.
+      (* Parameter types are well-formed *)
+      apply method_sig_wf_from_def with (m_sig := (msignature mdef)) in Hmdef_lookupcopy; auto.
+      destruct Hmdef_lookupcopy as [_ Hparams].
+      exact Hparams.
+
+      admit.
+      admit.
+    }
+    exact Hwf_method_frame.
+    rewrite -> Hbody_eq in Hmdef_lookup.
+    rewrite <- H2 in Hmdef_lookup.
+    exact Hmdef_lookup. 
+    unfold wf_r_config in Hwf.
+    destruct Hwf as [Hwf_classtable _].
+    exact Hwf_classtable.
+  }
+  - (* FldWrite: h' = update_field h lx f v2 *)
+  intros.
+  rewrite H3.
+  unfold update_field.
+  rewrite H0.
+  rewrite update_length.
+  reflexivity.
+  -
+  intros.
+  rewrite H5.
+  rewrite length_app.
+  simpl.
+  lia.
+  - (* Seq *)
+    intros.
+    inversion Hstmttyping; subst.
+        (* specialize (IHHeval1 eq_refl sΓ'0 sΓ Hwf H3) as IH1.
+    specialize (IHHeval2 eq_refl sΓ' sΓ'0 IH1 H5) as IH2. *)
+    apply Nat.le_trans with (dom h').
+    + (* Apply strong IH to first statement *)
+      apply IHHeval1 with (sΓ:=sΓ) (sΓ':=sΓ'0).
+      reflexivity.
+      exact Hwf.
+      exact H3.
+    + (* Apply strong IH to second statement *)
+      intros.
+      apply IHHeval2 with (sΓ:=sΓ'0) (sΓ':=sΓ').
+      reflexivity.
+      admit. (* somehow need the preservation...*)
+      exact H5.
+Admitted. *)
+
+(* Theorem readonly_pico :
+    forall CT sΓ rΓ h stmt rΓ' h' sΓ' l C vals vals' f qt readonlyx anyf rhs lhs anymethod anyrq,
+      stmt = (SFldWrite readonlyx anyf rhs) \/ stmt =  SCall lhs anymethod readonlyx [] -> 
+      static_getType sΓ readonlyx = Some qt ->
+      (* This is the interesting part, I think I have to supply empty arguments or all arguments as immutable because otherwise I don't if the readonly receiver is aliased with some mutable part *)
+      wf_r_config CT sΓ rΓ h ->
+      stmt_typing CT sΓ stmt sΓ' -> 
+      eval_stmt OK rΓ h stmt OK rΓ' h' -> 
+      runtime_getVal rΓ readonlyx = Some (Iot l)  ->
+      runtime_getObj h l = Some (mkObj (mkruntime_type anyrq C) vals) ->
+      runtime_getObj h' l = Some (mkObj (mkruntime_type anyrq C) vals') ->
+      sf_assignability_rel CT C f Final \/ sf_assignability_rel CT C f RDA ->
+      nth_error vals f = nth_error vals' f. *)
+      (*This looks like shallow mutability to me, but my language does not allow x.f1.f2 = y.*)
+
+(* Inductive reachability : heap -> Loc -> Loc -> Prop :=
+
+(* we can access the current location *)
+| rch_heap:
+    forall l h,
+      l < dom h ->
+      reachability h l l
+
+(* we can access a location in the local environment of the object at l0 *)
+| rch_step:
+    forall l0 l1 f obj v loc h,
+      l1 < dom h ->
+      getObj h l0 = Some obj ->
+      getVal obj.(fields_map) f = Some v -> 
+      v = Iot loc ->
+      loc = l1 ->
+      reachability h l0 l1
+
+(* transitive case *)
+| rch_trans:
+    forall l0 l1 l2 h,
+      reachability h l0 l1 ->
+      reachability h l1 l2 ->
+      reachability h l0 l2.
+Global Hint Constructors reachability: rch. *)
+
+(* Field is in the abstract state if it is qualified by Immut/RDM and Final/RDA *)
+(* Reachability by the abstract state *)
+(* Inductive reach_by_abstract_state: class_table -> heap -> s_env -> r_env -> Loc -> Loc -> Prop :=
+| rch_abs_heap:
+    forall ct l h sΓ rΓ,
+      l < dom h ->
+      reach_by_abstract_state ct h sΓ rΓ l l
+| rch_abs_step:
+    forall ct l0 l1 c f obj v qf loc h sΓ rΓ,
+      l1 < dom h ->
+      getObj h l0 = Some obj ->
+      getVal obj.(fields_map) f = Some v -> 
+      v = Iot loc ->
+      loc = l1 ->
+      r_basetype h l0 = Some c -> (* Base type of the object at l0 is c *)
+      sf_mutability ct c f = Some qf ->
+      q_f_proj qf = Imm /\ q_f_proj qf = RDM -> (* Mutability of field is either Imm or RDM *)
+      sf_assignability ct c f = Some Final /\ sf_assignability ct c f = Some RDA -> (* Field is Final/RDA *)
+      reach_by_abstract_state ct h sΓ rΓ l0 l1
+| rch_abstract_state_trans:
+    forall ct l0 l1 l2 h sΓ rΓ,
+      reach_by_abstract_state ct h sΓ rΓ l0 l1 ->
+      reach_by_abstract_state ct h sΓ rΓ l1 l2 ->
+      reach_by_abstract_state ct h sΓ rΓ l0 l2.
+Global Hint Constructors reach_by_abstract_state: rch_abs. *)
+
+(* Inductive abstract_equality : class_table -> heap -> s_env -> r_env -> Loc -> Loc -> Prop :=
+| abs_eq_refl:
+    forall ct h sΓ rΓ l,
+      l < dom h ->
+      abstract_equality ct h sΓ rΓ l l
+| abs_eq_fields :
+    forall ct h sΓ rΓ l0 l1 obj0 obj1 f v0 v1 loc0 loc1,
+      l1 < dom h ->
+      getObj h l0 = Some obj0 ->
+      getObj h l1 = Some obj1 ->
+      getVal obj0.(fields_map) f = Some v0 ->
+      getVal obj1.(fields_map) f = Some v1 ->
+      v0 = Null_a /\ v1 = Null_a \/
+      v0 = Iot loc0 /\ v1 = Iot loc1 /\ abstract_equality ct h sΓ rΓ loc0 loc1
+       ->
+      abstract_equality ct h sΓ rΓ l0 l1. *)
+
+(* Fixpoint vpa_assignability_by_loc: h -> l0 -> l1     *)
+(* Inductive vpa_assign_reachability : heap -> Loc -> Loc -> a -> Prop :=
+
+(* we can access the current location *)
+| rch_heap:
+    forall l h a,
+      l < dom h ->
+      reachability h l l a
+
+(* we can access a location in the local environment of the object at l0 *)
+| rch_step:
+    forall l0 l1 f obj q v loc h a,
+      l1 < dom h ->
+      getObj h l0 = Some obj ->
+      obj.(rt_type) = q ->
+      vpa_assignability (q_r_proj q) a = Assignable ->
+      getVal obj.(fields_map) f = Some v -> 
+      v = Iot loc ->
+      loc = l1 ->
+      reachability h l0 l1
+
+(* transitive case *)
+| rch_trans:
+    forall l0 l1 l2 h,
+      reachability h l0 l1 ->
+      reachability h l1 l2 ->
+      reachability h l0 l2. *)
+
+(* Lemma reachable_abs_object_unassignable_by_readonly_reference: *)
+
+(* Lemma reachable_abs_object_unassignable_for_immutable_object:
+  forall ct h sΓ rΓ l0 l1:
+    reach_by_abstract_state ct h sΓ rΓ l0 l1 -> *)
+
+
+    (* Method def lookup *)
+(* Fixpoint mdef_lookup (fuel : nat) (CT : class_table) (C : class_name) (m : method_name) : option method_def :=
+  match fuel with
+  | O => None
+  | S fuel' =>
+    match find_class CT C with
+    | None => None
+    | Some def =>
+      match find (fun mdef => eq_method_name (mname (msignature mdef)) m)
+                 (methods (body def)) with
+      | Some mdef => Some mdef
+      | None =>
+        match super (signature def) with
+        | None => None
+        | Some superC => mdef_lookup fuel' CT superC m
+        end
+      end
+    end
+  end. *)
+
+(* Method definition lookup  *)
+(* Definition method_def_lookup (CT : class_table) (C : class_name) (m : method_name) : option method_def :=
+  mdef_lookup (length CT) CT C m. *)
+
+(* Method signature lookup *)
+(* Definition method_sig_lookup (CT : class_table) (C : class_name) (m : method_name) : option (method_sig) :=
+  match mdef_lookup (length CT) CT C m with
+  | Some mdef => Some mdef.(msignature)
+  | None => None
+  end. *)
+
+(* Method body lookup *)
+(* Definition method_body_lookup (CT : class_table) (C : class_name) (m : method_name) : option method_body :=
+  match mdef_lookup (length CT) CT C m with
+  | Some mdef => Some mdef.(mbody)
+  | None => None
+  end. *)
+
+(* Lemma method_body_lookup_implies_sig_lookup : forall CT C m mbody,
+  method_body_lookup CT C m = Some mbody ->
+  exists msig, method_sig_lookup CT C m = Some msig.
+Proof.
+  intros CT C m mbody H.
+  unfold method_body_lookup in H.
+  unfold method_sig_lookup.
+  destruct (mdef_lookup (length CT) CT C m) as [mdef|] eqn:Hmdef.
+  - injection H as H_eq. subst mbody.
+    exists (msignature mdef).
+    reflexivity.
+  - discriminate H.
+Qed.
+
+Lemma method_body_lookup_implies_def_lookup : forall CT C m mebody,
+  method_body_lookup CT C m = Some mebody ->
+  exists mdef, method_def_lookup CT C m = Some mdef /\ (mbody mdef) = mebody.
+Proof.
+  intros CT C m mebody H.
+  unfold method_body_lookup in H.
+  unfold method_def_lookup.
+  destruct (mdef_lookup (length CT) CT C m) as [mdef|] eqn:Hmdef.
+  - injection H as H_eq. subst mebody.
+    exists mdef.
+    split.
+    + reflexivity.
+    + reflexivity.
+  - discriminate H.
+Qed.
+
+Lemma method_sig_lookup_implies_body_lookup : forall CT C m msig,
+  method_sig_lookup CT C m = Some msig ->
+  exists mbody, method_body_lookup CT C m = Some mbody.
+Proof.
+  intros CT C m msig H.
+  unfold method_sig_lookup in H.
+  unfold method_body_lookup.
+  destruct (mdef_lookup (length CT) CT C m) as [mdef|] eqn:Hmdef.
+  - injection H as H_eq. subst msig.
+    exists (mbody mdef).
+    reflexivity.
+  - discriminate H.
+Qed. *)
+
+(* Definition find_overriding_method (CT : class_table) (C: class_name) (m: method_sig) : option method_sig :=
+  match mdef_lookup (length CT) CT C (mname m) with
+  | Some mdef =>
+      let msig := msignature mdef in
+      if eq_method_name (mname msig) (mname m)
+         (* && forallb2 (fun C1 C2 =>
+          eq_class_name C1.(sctype) C2.(sctype)
+         ) (mparams msig) (mparams m)
+         && eq_class_name (sctype (mret msig)) (sctype (mret m)) *)
+      then Some msig
+      else None
+  | None => None
+  end. *)
+
+  (* Lemma method_frame_wf_r_config : forall CT sΓ rΓ h y ly Ty vals mdef m_sig args argtypes C m,
+  wf_r_config CT sΓ rΓ h ->
+  C < dom CT ->
+  runtime_getVal rΓ y = Some (Iot ly) ->
+  static_getType sΓ y = Some Ty ->
+  runtime_lookup_list rΓ args = Some vals ->
+  static_getType_list sΓ args = Some argtypes ->
+  MethodLookup CT C m mdef ->
+  m_sig = msignature mdef ->
+  qualified_type_subtype CT Ty (vpa_qualified_type (sqtype Ty) (mreceiver m_sig)) ->
+  Forall2 (fun arg T => qualified_type_subtype CT arg (vpa_qualified_type (sqtype Ty) T)) 
+          argtypes (mparams m_sig) ->
+  wf_r_config CT (mreceiver m_sig :: mparams m_sig) 
+              {| vars := Iot ly :: vals |} h.
+Proof.
+  intros.
+  unfold wf_r_config.
+  repeat split.
+  destruct H as [Hclass [Hheap [Hrenv [Hsenv [Hlen Hcorr]]]]].
+  unfold wf_class_table in Hclass.
+  destruct Hclass as [Hclass [Hobj [Hotherclasses Hcname_consistent]]].
+  exact Hclass.
+  destruct H as [Hclass [Hheap [Hrenv [Hsenv [Hlen Hcorr]]]]].
+  destruct Hclass as [Hclass [Hobj [Hotherclasses Hcname_consistent]]].
+  exact Hobj.
+  destruct H as [Hclass [Hheap [Hrenv [Hsenv [Hlen Hcorr]]]]].
+  destruct Hclass as [Hclass [Hobj [Hotherclasses Hcname_consistent]]].
+  exact Hotherclasses.
+  destruct H as [Hclass [Hheap [Hrenv [Hsenv [Hlen Hcorr]]]]].
+  destruct Hclass as [Hclass [Hobj [Hotherclasses Hcname_consistent]]].
+  apply Hcname_consistent.
+  destruct H as [Hclass [Hheap [Hrenv [Hsenv [Hlen Hcorr]]]]].
+  destruct Hclass as [Hclass [Hobj [Hotherclasses Hcname_consistent]]].
+  apply Hcname_consistent.
+
+  destruct H as [Hclass [Hheap [Hrenv [Hsenv [Hlen Hcorr]]]]].
+  exact Hheap.
+  simpl.
+  lia.
+
+  {
+    exists ly.
+    split.
+    simpl.
+    reflexivity.
+    destruct H as [_ [_ [_ [_ [_ Hcorr]]]]].
+    specialize (Hcorr y).
+    assert (Hy_dom : y < dom sΓ).
+    { apply static_getType_dom in H2. exact H2. }
+    specialize (Hcorr Hy_dom Ty H2).
+    rewrite H1 in Hcorr.
+    unfold wf_r_typable in Hcorr.
+    destruct (r_type h ly) as [rqt|] eqn:Hrtype; [|contradiction].
+    apply r_type_dom in Hrtype.
+    exact Hrtype.
+  }
+
+  {
+    simpl.
+    constructor.
+    simpl.
+    destruct H as [_ [_ [_ [_ [_ Hcorr]]]]].
+    specialize (Hcorr y).
+    assert (Hy_dom : y < dom sΓ).
+    { apply static_getType_dom in H2. exact H2. }
+    specialize (Hcorr Hy_dom Ty H2).
+    rewrite H1 in Hcorr.
+    unfold wf_r_typable in Hcorr.
+    destruct (r_type h ly) as [rqt|] eqn:Hrtype; [|contradiction].
+    unfold r_type in Hrtype.
+    destruct (runtime_getObj h ly) as [obj|] eqn:Hobj; [trivial | discriminate].
+    assert (H_forall: Forall (fun value => match value with
+      | Null_a => True
+      | Iot loc => match runtime_getObj h loc with Some _ => True | None => False end
+      end) vals).
+    {
+      eapply runtime_lookup_list_preserves_wf_values; eauto.
+      unfold wf_r_config in H.
+      destruct H as [_ [_ [Hrenv _]]].
+      unfold wf_renv in Hrenv.
+      destruct Hrenv as [Hrenvdom [Hreceiver Hforall]].
+      (* destruct Hreceiver as [Hreceiverval Hreceivervaldom]. *)
+      unfold wf_renv.
+      repeat split.
+      - (* dom (vars rΓ) > 0 *)
+        exact Hrenvdom.
+      - (* exists iot, gget (vars rΓ) 0 = Some (Iot iot) /\ iot < dom h *)
+        exact Hreceiver.
+      - (* Forall well-formed values *)
+        exact Hforall.
+    }
+    exact H_forall.
+  }
+
+  {
+    simpl. lia.
+  }
+
+  {
+    constructor.
+      destruct H as [Hclass _].
+      apply method_sig_wf in H5; auto.
+      destruct H5 as [Hreceiver _].
+      rewrite H6.
+      exact Hreceiver.
+      destruct H as [Hclass _].
+      apply method_sig_wf in H5; auto.
+      destruct H5 as [_ Hparams].
+      rewrite H6.
+      exact Hparams.
+  }
+
+  {
+    simpl.
+    f_equal.
+    apply Forall2_length in H8.
+    apply static_getType_list_preserves_length in H4.
+    apply runtime_lookup_list_preserves_length in H3.
+    rewrite -> H4 in H8.
+    rewrite <- H3 in H8.
+    symmetry.
+    exact H8.
+  }
+  {
+    intros i Hi sqt Hnth.
+    destruct i as [|i'].
+    - (* Case: i = 0 (receiver) *)
+      simpl in Hnth.
+      injection Hnth as Heq. subst sqt.
+      simpl.
+      unfold wf_r_typable.
+      destruct H as [Hclasstable [Hheap [_ [Hsenv [_ Hcorr]]]]].
+      specialize (Hcorr y).
+      assert (Hy_dom : y < dom sΓ).
+      { apply static_getType_dom in H2. exact H2. }
+      specialize (Hcorr Hy_dom Ty H2).
+      rewrite H1 in Hcorr.
+
+      eapply wf_r_typable_subtype; eauto.
+      apply senv_var_domain with (sΓ := sΓ) (i := y); auto.
+      unfold static_getType in H2.
+      exact H2.
+
+      apply method_sig_wf in H5; auto.
+      destruct H5 as [Hreceiver _].
+      unfold wf_stypeuse in Hreceiver.
+      destruct (bound CT (sctype (mreceiver (msignature mdef)))) as [q_bound|] eqn:Hbound; [|contradiction].
+      destruct Hreceiver as [_ Hdom].
+      rewrite H6.
+      exact Hdom.
+
+      unfold wf_r_typable in Hcorr |- *.
+      destruct (r_type h ly) as [rqt|] eqn:Hrtype; [|contradiction].
+      destruct (get_this_var_mapping (vars {| vars := Iot ly :: vals |})) as [ι'|] eqn:Hthis.
+      simpl in Hthis.
+      injection Hthis as Hthis_eq.
+      subst ι'.
+      destruct (r_muttype h ly) as [q|] eqn:Hmut.
+      destruct (get_this_var_mapping (vars rΓ)) as [ι'|] eqn:Hthis_orig; [|contradiction].
+      destruct (r_muttype h ι') as [q_orig|] eqn:Hmut_orig; [|contradiction].
+      (* exact Hcorr. Continue later *)
+      admit.
+
+      exfalso.
+      unfold r_type in Hrtype.
+      unfold r_muttype in Hmut.
+      destruct (runtime_getObj h ly) as [obj|] eqn:Hobj; [|discriminate].
+      destruct (get_this_var_mapping (vars rΓ)) as [this|] eqn:Hthis; [|discriminate].
+      discriminate.
+
+      exfalso.
+      simpl in Hthis.
+      discriminate.
+      admit.
+
+    - (* Case: i = S i' (parameters) *)
+      simpl in Hnth.
+      assert (Hi'_bound : i' < dom (mparams m_sig)).
+      { simpl in Hi. lia. }
+      assert (Hparam_nth : nth_error (mparams m_sig) i' = Some sqt).
+      { exact Hnth. }
+      simpl.
+      (* Get the corresponding argument type and value *)
+      assert (Hi'_args : i' < dom args).
+      {
+        apply Forall2_length in H8.
+        apply static_getType_list_preserves_length in H4.
+        apply runtime_lookup_list_preserves_length in H3.
+        rewrite -> H4 in H8.
+        rewrite <- H8 in Hi'_bound.
+        exact Hi'_bound.
+      }
+      admit. (* Complex proof involving parameter correspondence *)
+  }
+Admitted. *)
