README.md
@@ -16,3 +16,13 @@
    ```sh
    make
    ```
+## Ideas on refactoring
+
+1. Remove cname and just use the indice. This will simpfy the encoding of wf_class_table.
+2. Define explict object type and simpfy the wf_class, method and constructor.
+3. Define seperate runtime qualifier and use tyable relation between runtime qualifier and static type instead. It is somehow hacky to do what I am doing now for lost. [fixed]
+4. This proof currently is on relationship big-step semantics, there were also functional big-step semantics, pretty big-step semantics and coinductive big-step semantics.
+5. learning: fixpoint and inductive's proof
+6. learnng: projectection is hard and bad.
+7. learning: complex case analysis (more than 600 cases).
+8. doing induction over the evaluation rule if there is subterm
